

$$\begin{array}{c}
 \begin{matrix} r3 \\ \hline \hline \end{matrix} \left[\begin{array}{c} \hline \hline \end{array} \right] \begin{matrix} c4 \\ \hline \hline \end{matrix} \left[\begin{array}{c} \hline \hline \end{array} \right] = \left[\begin{array}{c} c_{34} \\ \hline \hline \end{array} \right] \\
 A (m \times n) \quad B (n \times p) \quad C = AB (m \times p)
 \end{array}$$

$$C_{34} = (\text{row 3 of } A) \times (\text{col 4 of } B)$$

$$= a_{31} \cdot b_{14} + a_{32} \cdot b_{24} + \dots = \sum_{k=1}^n a_{3k} b_{k4}$$

$$\begin{array}{c}
 \left[\begin{array}{c} \hline \hline \hline \hline \hline \hline \end{array} \right] \left[\begin{array}{c} \hline \hline \hline \hline \hline \hline \end{array} \right] = \left[\begin{array}{c} \hline \hline \hline \hline \hline \hline \end{array} \right] \\
 A \quad B \quad C \\
 (m \times n) \quad (n \times p) \quad (m \times p)
 \end{array}$$

\Downarrow

* columns of C are combinations of columns of A

* rows of C are combinations of rows of B

column of A \times row of B
 $(m \times 1)$ $(1 \times p)$

$$\begin{bmatrix} 1 \\ 2 \\ 3 \end{bmatrix} \begin{bmatrix} 2 & 4 \end{bmatrix} = \begin{bmatrix} 2 & 4 \\ 4 & 8 \\ 6 & 12 \end{bmatrix}$$

$\ast AB = \text{sum of } \{(\text{cols of A}) \times (\text{rows of B})\}$

$$\begin{bmatrix} 2 & 5 \\ 3 & 6 \\ 4 & 7 \end{bmatrix} \begin{bmatrix} 1 & 2 \\ 3 & 4 \end{bmatrix}$$

$$= \begin{bmatrix} 2 \\ 3 \\ 4 \end{bmatrix} \begin{bmatrix} 1 & 2 \end{bmatrix} + \begin{bmatrix} 5 \\ 6 \\ 7 \end{bmatrix} \begin{bmatrix} 3 & 4 \end{bmatrix}$$

Block Multiplication

$$\begin{array}{c} \begin{bmatrix} A_1 & A_2 \\ A_3 & A_4 \end{bmatrix} \\ A \end{array} \begin{array}{c} \begin{bmatrix} B_1 & B_2 \\ B_3 & B_4 \end{bmatrix} \\ B \end{array} = \begin{bmatrix} & \\ & \end{bmatrix}$$

$A_1 B_1 + A_2 B_3$

INVERSES (square)

$$\textcircled{A^{-1}} A = I = A A^{-1}$$

if this exists... \rightarrow invertible, non-singular

[singular / no inverse]

$$A = \begin{bmatrix} 1 & 3 \\ 2 & 6 \end{bmatrix}$$

I can find a vector $x \neq 0$
with $Ax = 0$

$$\begin{bmatrix} \\ \end{bmatrix}_A \begin{bmatrix} 3 \\ -1 \end{bmatrix} = \begin{bmatrix} 0 \\ 0 \end{bmatrix}$$

[non-singular]

$$\begin{bmatrix} 1 & 3 \\ 2 & 7 \end{bmatrix}_A \begin{bmatrix} a & c \\ b & d \end{bmatrix}_{A^{-1}} = \begin{bmatrix} 1 & 0 \\ 0 & 1 \end{bmatrix}_I$$

$A \times \text{column } j \text{ of } A^{-1} = \text{column } j \text{ of } I$

[Gauss-Jordan]

solve two equation at once

$$\begin{bmatrix} 1 & 3 \\ 2 & 7 \end{bmatrix} \begin{bmatrix} a \\ b \end{bmatrix} = \begin{bmatrix} 1 \\ 0 \end{bmatrix}$$

$$\begin{bmatrix} 1 & 3 \\ 2 & 7 \end{bmatrix} \begin{bmatrix} 0 \\ 1 \end{bmatrix} = \begin{bmatrix} 0 \\ 1 \end{bmatrix}$$

$$\rightarrow \left[\begin{array}{cc|cc} 1 & 3 & 1 & 0 \\ 2 & 7 & 0 & 1 \end{array} \right] \rightarrow \left[\begin{array}{cc|cc} 1 & 3 & 1 & 0 \\ 0 & 1 & -2 & 1 \end{array} \right]$$

$A \qquad I$

$$\rightarrow \left[\begin{array}{cc|cc} 1 & 0 & 7 & -3 \\ 0 & 1 & -2 & 1 \end{array} \right]$$

$I \qquad A^{-1}$

It's $[A \ I] =$

$[I, ?]$

$$\left[\begin{array}{ll} EA = I & E = A^{-1} \\ EI = ? & ? = E = A^{-1} \end{array} \right]$$